Use ghost map for bumpers

src/high/resources/bumpers.v
@@ -1,5 +1,5 @@
-From iris.algebra Require Import gmap auth.
-From iris.base_logic.lib Require Import own.
+From iris.algebra Require Import gmap auth gmap_view.
+From iris.base_logic.lib Require Import own ghost_map.
 From iris.heap_lang Require Export locations.
 From iris.proofmode Require Import proofmode.
 
@@ -7,51 +7,68 @@ From self Require Import extra.
 From self.high Require Import abstract_state.
 
 Definition bumpersR :=
-  authR (gmapUR loc (agreeR (leibnizO (positive → option positive)))).
+  (* authR (gmapUR loc (agreeR (leibnizO (positive → option positive)))). *)
+  gmap_viewR loc (leibnizO (positive → option positive)).
+
+Notation bumpersG Σ := (ghost_mapG Σ loc (positive → option positive)).
 
 Section bumpers.
-  Context `{inG Σ bumpersR}.
+  Context `{bumpersG Σ}.
   Context `{AbstractState ST}.
 
+  Definition encode_bumper (bumper : ST → ST) :=
+    λ e, encode <$> (bumper <$> decode e).
+
   Definition own_know_bumper γ (ℓ : loc) (bumper : ST → ST) : iProp Σ :=
-    let encodedBumper e := encode <$> (bumper <$> decode e)
+    let encodedBumper := encode_bumper bumper
     in ⌜∀ s1 s2, s1 ⊑ s2 → bumper s1 ⊑ bumper s2⌝ ∗
-       own γ ((◯ {[ ℓ := to_agree encodedBumper ]}) : bumpersR).
+       ℓ ↪[γ]□ encodedBumper.
+       (* own γ ((◯ {[ ℓ := to_agree encodedBumper ]}) : bumpersR). *)
 
   Definition own_all_bumpers γ encoded_bumpers :=
-    own γ (● (to_agree <$> encoded_bumpers) : bumpersR).
+    ghost_map_auth γ (1) encoded_bumpers.
+    (* own γ (● (to_agree <$> encoded_bumpers) : bumpersR). *)
 
   (* Definition own_all_bumpers encoded_bumpers := *)
   (*   own_all_bumpers bumpers_name encoded_bumpers. *)
 
   Lemma own_all_bumpers_alloc bumpers :
     ⊢ |==> ∃ γ, own_all_bumpers γ bumpers ∗
-                own γ (◯ ((to_agree <$> bumpers) : gmapUR _ (agreeR _))).
+                ([∗ map] ℓ ↦ bumper ∈ bumpers, ℓ ↪[γ]□ bumper).
   Proof.
-    setoid_rewrite <- own_op.
-    iApply own_alloc.
-    apply auth_both_valid_discrete. split; first done.
-    apply valid_to_agree_fmap.
-  Qed.
+    (* TODO: Add some more lemmas to ghost_map that will make this easy. *)
+  Admitted.
+  (*   (* iApply ghost_map_alloc. *) *)
+  (* Qed. *)
 
-  Lemma own_all_bumpers_persist γ encoded_bumpers :
-    own_all_bumpers γ encoded_bumpers ==∗
-    own γ (●□ ((to_agree <$> encoded_bumpers) : gmapUR _ (agreeR _))).
-  Proof. iApply own_update. apply auth_update_auth_persist. Qed.
+  (* Lemma own_all_bumpers_persist γ encoded_bumpers : *)
+  (*   own_all_bumpers γ encoded_bumpers ==∗ *)
+  (*   own γ (●□ ((to_agree <$> encoded_bumpers) : gmapUR _ (agreeR _))). *)
+  (* Proof. iApply own_update. apply auth_update_auth_persist. Qed. *)
 
-  Lemma bumpers_frag_lookup γ (bumpers : gmap loc (positive → option positive))
-        (ℓ : loc) (bumper : positive → option positive) :
-    bumpers !! ℓ = Some bumper →
-    own γ (◯ (to_agree <$> bumpers) : bumpersR) -∗
-    own γ (◯ {[ ℓ := to_agree bumper ]}).
+  (* Lemma bumpers_frag_extract γ (bumpers : gmap loc (positive → option positive)) *)
+  (*       (ℓ : loc) (bumper : positive → option positive) : *)
+  (*   bumpers !! ℓ = Some bumper → *)
+  (*   own γ (◯ (to_agree <$> bumpers) : bumpersR) -∗ *)
+  (*   own γ (◯ {[ ℓ := to_agree bumper ]}). *)
+  (* Proof. *)
+  (*   intros look. f_equiv. simpl. *)
+  (*   apply auth_frag_mono. *)
+  (*   rewrite singleton_included_l. *)
+  (*   eexists _. *)
+  (*   rewrite lookup_fmap look. *)
+  (*   naive_solver. *)
+  (* Qed. *)
+
+  Definition bumperO := leibnizO (positive → option positive).
+
+  Lemma bumpers_lookup γ ℓ encoded_bumpers bumper :
+    own_all_bumpers γ encoded_bumpers -∗
+    own_know_bumper γ ℓ bumper -∗
+    ⌜ encoded_bumpers !! ℓ = Some (encode_bumper bumper) ⌝.
   Proof.
-    intros look. f_equiv. simpl.
-    apply auth_frag_mono.
-    rewrite singleton_included_l.
-    eexists _.
-    rewrite lookup_fmap look.
-    naive_solver.
+    iIntros "A [mono F]".
+    iDestruct (ghost_map_lookup with "A F") as "$".
   Qed.
 
 End bumpers.
-
